example/CaseStudyHuttonsRazor/RazorProofsMaybe.v
@@ -1,79 +1,10 @@
-From Base Require Import Free Free.Instance.Maybe Free.Instance.Error Prelude Test.QuickCheck.
-From Generated Require Import Proofs.Razor.
+From Base Require Import Free Free.Instance.Maybe Prelude.
+From Extra Require Import ExprInd Tactic.
+From Generated Require Import Razor.
+From Proofs Require Import AppendAssocProofs.
 
 Require Import Coq.Logic.FunctionalExtensionality.
 Require Import Coq.Program.Equality.
-
-(* Define some additional tactics. *)
-Ltac simplifyInductionHypothesis ident1 ident2 :=
-  match goal with
-  | [ ident1 : ForFree ?Shape ?Pos ?A ?P (pure _) |- _ ] => inversion ident1 as [ Heq ident2 |]; clear ident1; subst Heq; simpl
-  | [ ident1 : ForFree ?Shape ?Pos ?A ?P (impure ?s ?pf) |- _ ] =>
-    dependent destruction ident1;
-    match goal with
-    | [ H1 : forall p : ?T, ForFree ?Shape ?Pos ?A ?P (?pf p), H0 : forall p, ForFree ?Shape ?Pos ?A ?Py (?pf p) -> _ = _,
-        p : ?T |- _ ] =>
-      specialize (H0 p (H1 p)) as ident2; clear H1; clear H0; simpl
-    end
-  end.
-
-Tactic Notation "simplify'" ident(H) "as" ident(IH) := (simplifyInductionHypothesis H IH).
-
-Ltac autoInductionHypothesis :=
-  match goal with
-  (*  | [ s : Zero__S |- _ ] => destruct s *)
-  | [ H : ForFree ?Shape ?Pos ?A ?P (impure ?s ?pf) |- ?h ?s ?pf1 = ?h ?s ?pf2 ] =>
-    f_equal; let x := fresh in
-             extensionality x; simplify' H as Hnew; assumption
-    (*   try apply newH) *)
-  | [ H : ForFree ?Shape ?Pos ?A ?P (pure ?x) |- _ ] =>
-    let newH := fresh in simplify' H as newH; rename newH into IH
-  | [ H : forall p : ?T, ?f = ?g |- ?h ?s ?pf1 = ?h ?s ?pf2 ] =>
-    f_equal; let x := fresh in extensionality x; apply H
-  | [ H : forall p : ?T, ?f = ?g |- impure ?s ?pf1 = impure ?s ?pf2 ] =>
-    f_equal; let x := fresh in extensionality x; apply H
-  end.
-
-Tactic Notation "autoIH" := (autoInductionHypothesis).
-
-Tactic Notation "inductFree" ident(fx) "as" simple_intropattern(pat) := (induction fx as pat; simpl; try autoIH).
-
-(* Define induction scheme for [Expr]. *)
-Section Expr_ind.
-
-  Variable Shape : Type.
-  Variable Pos   : Shape -> Type.
-  Variable P     : Expr Shape Pos -> Prop.
-
-  Hypothesis valP : forall (fn : Free Shape Pos (Integer.Integer Shape Pos)), P (val fn).
-
-  Hypothesis addP : forall (fx fy : Free Shape Pos (Expr Shape Pos)),
-    ForFree Shape Pos (Expr Shape Pos) P fx ->
-      ForFree Shape Pos (Expr Shape Pos) P fy ->
-        P (add0 fx fy).
-
-  Fixpoint Expr_Ind (expr : Expr Shape Pos) : P expr.
-  Proof.
-    destruct expr as [ fn | fx fy ].
-    - apply valP.
-    - apply addP.
-      + apply ForFree_forall. intros e IHe.
-        inductFree fx as [ x | s pf IHpf ].
-        * inversion IHe; subst. apply Expr_Ind.
-        * dependent destruction IHe; subst. destruct H as [ p ].
-          apply IHpf with (p := p). apply H.
-      + apply ForFree_forall. intros e IHe.
-        inductFree fy as [ y | s pf IHpf ].
-        * inversion IHe; subst. apply Expr_Ind.
-        * dependent destruction IHe; subst. destruct H as [ p ].
-          apply IHpf with (p := p). apply H.
-  Defined.
-
-End Expr_ind.
-
-(* The following lemma and theorem are proven in the file `AppendAssocProofs.v`. *)
-Lemma append_nil : quickCheck prop_append_nil. Proof. Admitted.
-Theorem append_assoc : quickCheck prop_append_assoc. Proof. Admitted.
 
 Section Proofs_Maybe.
 
