example/CaseStudyHuttonsRazor/Extra/ExprInd.v
@@ -1,0 +1,36 @@
+From Base Require Import Free.
+From Generated Require Import Razor.
+
+Require Import Coq.Program.Equality.
+
+Section Expr_ind.
+
+  Variable Shape : Type.
+  Variable Pos   : Shape -> Type.
+  Variable P     : Expr Shape Pos -> Prop.
+
+  Hypothesis valP : forall (fn : Free Shape Pos (Integer.Integer Shape Pos)), P (val fn).
+
+  Hypothesis addP : forall (fx fy : Free Shape Pos (Expr Shape Pos)),
+    ForFree Shape Pos (Expr Shape Pos) P fx ->
+      ForFree Shape Pos (Expr Shape Pos) P fy ->
+        P (add0 fx fy).
+
+  Fixpoint Expr_Ind (expr : Expr Shape Pos) : P expr.
+  Proof.
+    destruct expr as [ fn | fx fy ].
+    - apply valP.
+    - apply addP.
+      + apply ForFree_forall. intros e IHe.
+        induction fx as [ x | s pf IHpf ] using Free_Ind.
+        * inversion IHe; subst. apply Expr_Ind.
+        * dependent destruction IHe; subst. destruct H as [ p ].
+          apply IHpf with (p := p). apply H.
+      + apply ForFree_forall. intros e IHe.
+        induction fy as [ y | s pf IHpf ] using Free_Ind.
+        * inversion IHe; subst. apply Expr_Ind.
+        * dependent destruction IHe; subst. destruct H as [ p ].
+          apply IHpf with (p := p). apply H.
+  Defined.
+
+End Expr_ind.
