example/CaseStudyHuttonsRazor/Output/Razor.v
@@ -1,0 +1,227 @@
+(* module Razor *)
+
+From Base Require Import Free.
+
+From Base Require Import Prelude.
+
+From Base Require Import Test.QuickCheck.
+
+From Generated Require Export Proofs.AppendAssoc.
+
+Definition Stack (Shape : Type) (Pos : Shape -> Type) : Type :=
+  List Shape Pos (Integer Shape Pos).
+
+(* Data type declarations for Op *)
+
+Inductive Op (Shape : Type) (Pos : Shape -> Type) : Type
+  := push : Free Shape Pos (Integer Shape Pos) -> Op Shape Pos
+  |  add : Op Shape Pos.
+
+(* Arguments sentences for Op *)
+
+Arguments push {Shape} {Pos}.
+
+Arguments add {Shape} {Pos}.
+
+(* Smart constructors for Op *)
+
+Definition PUSH (Shape : Type) (Pos : Shape -> Type) (x_0
+    : Free Shape Pos (Integer Shape Pos))
+   : Free Shape Pos (Op Shape Pos) :=
+  pure (push x_0).
+
+Definition ADD (Shape : Type) (Pos : Shape -> Type)
+   : Free Shape Pos (Op Shape Pos) :=
+  pure add.
+
+(* Data type declarations for Expr *)
+
+Inductive Expr (Shape : Type) (Pos : Shape -> Type) : Type
+  := val : Free Shape Pos (Integer Shape Pos) -> Expr Shape Pos
+  |  add0
+   : Free Shape Pos (Expr Shape Pos) ->
+     Free Shape Pos (Expr Shape Pos) -> Expr Shape Pos.
+
+(* Arguments sentences for Expr *)
+
+Arguments val {Shape} {Pos}.
+
+Arguments add0 {Shape} {Pos}.
+
+(* Smart constructors for Expr *)
+
+Definition Val (Shape : Type) (Pos : Shape -> Type) (x_0
+    : Free Shape Pos (Integer Shape Pos))
+   : Free Shape Pos (Expr Shape Pos) :=
+  pure (val x_0).
+
+Definition Add0 (Shape : Type) (Pos : Shape -> Type) (x_0
+    : Free Shape Pos (Expr Shape Pos)) (x_1 : Free Shape Pos (Expr Shape Pos))
+   : Free Shape Pos (Expr Shape Pos) :=
+  pure (add0 x_0 x_1).
+
+Definition Code (Shape : Type) (Pos : Shape -> Type) : Type :=
+  List Shape Pos (Op Shape Pos).
+
+(* Helper functions for exec *)
+
+Fixpoint exec_0 (Shape : Type) (Pos : Shape -> Type) (P : Partial Shape Pos) (a7
+                  : Code Shape Pos) (a8 : Free Shape Pos (Stack Shape Pos)) {struct a7} : Free
+                                                                                          Shape Pos (Stack Shape Pos)
+           := match a7 with
+              | nil =>
+                  a8 >>=
+                  (fun a8_3 =>
+                     match a8_3 with
+                     | nil => @Nil Shape Pos (Integer Shape Pos)
+                     | cons a9 a10 => @Cons Shape Pos (Integer Shape Pos) a9 a10
+                     end)
+              | cons a13 a14 =>
+                  a13 >>=
+                  (fun a13_0 =>
+                     match a13_0 with
+                     | push a21 =>
+                         a8 >>=
+                         (fun a8_3 =>
+                            match a8_3 with
+                            | nil =>
+                                a14 >>=
+                                (fun (a14_0 : Code Shape Pos) =>
+                                   exec_0 Shape Pos P a14_0 (@Cons Shape Pos (Integer Shape Pos) a21 (@Nil Shape
+                                                                                                  Pos (Integer Shape
+                                                                                                               Pos))))
+                            | cons a24 a25 =>
+                                a14 >>=
+                                (fun (a14_0 : Code Shape Pos) =>
+                                   exec_0 Shape Pos P a14_0 (@Cons Shape Pos (Integer Shape Pos) a21 (@Cons Shape
+                                                                                                  Pos (Integer Shape
+                                                                                                               Pos) a24
+                                                                                                                    a25)))
+                            end)
+                     | add =>
+                         a8 >>=
+                         (fun a8_3 =>
+                            match a8_3 with
+                            | cons a28 a29 =>
+                                a29 >>=
+                                (fun a29_0 =>
+                                   match a29_0 with
+                                   | cons a32 a33 =>
+                                       a14 >>=
+                                       (fun (a14_0 : Code Shape Pos) =>
+                                          exec_0 Shape Pos P a14_0 (@Cons Shape Pos (Integer Shape Pos) (addInteger
+                                                                                                         Shape Pos a32
+                                                                                                         a28) a33))
+                                   | nil => @undefined Shape Pos P (Stack Shape Pos)
+                                   end)
+                            | nil => @undefined Shape Pos P (Stack Shape Pos)
+                            end)
+                     end)
+              end.
+
+Definition exec (Shape : Type) (Pos : Shape -> Type) (P : Partial Shape Pos) (a7
+    : Free Shape Pos (Code Shape Pos)) (a8 : Free Shape Pos (Stack Shape Pos))
+   : Free Shape Pos (Stack Shape Pos) :=
+  a7 >>= (fun (a7_0 : Code Shape Pos) => exec_0 Shape Pos P a7_0 a8).
+
+(* Helper functions for eval *)
+
+Fixpoint eval_0 (Shape : Type) (Pos : Shape -> Type) (a0 : Expr Shape Pos)
+                {struct a0} : Free Shape Pos (Integer Shape Pos)
+           := match a0 with
+              | val a1 => a1
+              | add0 a3 a4 =>
+                  addInteger Shape Pos (a3 >>=
+                              (fun (a3_0 : Expr Shape Pos) => eval_0 Shape Pos a3_0)) (a4 >>=
+                              (fun (a4_0 : Expr Shape Pos) => eval_0 Shape Pos a4_0))
+              end.
+
+Definition eval (Shape : Type) (Pos : Shape -> Type) (a0
+    : Free Shape Pos (Expr Shape Pos))
+   : Free Shape Pos (Integer Shape Pos) :=
+  a0 >>= (fun (a0_0 : Expr Shape Pos) => eval_0 Shape Pos a0_0).
+
+(* Helper functions for compApp *)
+
+Fixpoint compApp_0 (Shape : Type) (Pos : Shape -> Type) (a43 : Expr Shape Pos)
+                   (a44 : Free Shape Pos (Code Shape Pos)) {struct a43} : Free Shape Pos (Code
+                                                                                Shape Pos)
+           := match a43 with
+              | val a45 => @Cons Shape Pos (Op Shape Pos) (PUSH Shape Pos a45) a44
+              | add0 a47 a48 =>
+                  a47 >>=
+                  (fun (a47_0 : Expr Shape Pos) =>
+                     compApp_0 Shape Pos a47_0 (a48 >>=
+                                (fun (a48_0 : Expr Shape Pos) =>
+                                   compApp_0 Shape Pos a48_0 (@Cons Shape Pos (Op Shape Pos) (ADD Shape Pos)
+                                                                                             a44))))
+              end.
+
+Definition compApp (Shape : Type) (Pos : Shape -> Type) (a43
+    : Free Shape Pos (Expr Shape Pos)) (a44 : Free Shape Pos (Code Shape Pos))
+   : Free Shape Pos (Code Shape Pos) :=
+  a43 >>= (fun (a43_0 : Expr Shape Pos) => compApp_0 Shape Pos a43_0 a44).
+
+Definition comp' (Shape : Type) (Pos : Shape -> Type) (e
+    : Free Shape Pos (Expr Shape Pos))
+   : Free Shape Pos (Code Shape Pos) :=
+  compApp Shape Pos e (@Nil Shape Pos (Op Shape Pos)).
+
+Definition prop_comp'_correct (Shape : Type) (Pos : Shape -> Type) (P
+    : Partial Shape Pos) (e : Free Shape Pos (Expr Shape Pos))
+   : Free Shape Pos (Property Shape Pos) :=
+  @eqProp Shape Pos (Stack Shape Pos) (exec Shape Pos P (comp' Shape Pos e) (@Nil
+                                             Shape Pos (Integer Shape Pos))) (@Cons Shape Pos (Integer Shape Pos) (eval
+                                                                                                                   Shape
+                                                                                                                   Pos
+                                                                                                                   e)
+                                                                                                                  (@Nil
+                                                                                                                   Shape
+                                                                                                                   Pos
+                                                                                                                   (Integer
+                                                                                                                    Shape
+                                                                                                                    Pos))).
+
+(* Helper functions for comp *)
+
+Fixpoint comp_0 (Shape : Type) (Pos : Shape -> Type) (a36 : Expr Shape Pos)
+                {struct a36} : Free Shape Pos (Code Shape Pos)
+           := match a36 with
+              | val a37 =>
+                  @Cons Shape Pos (Op Shape Pos) (PUSH Shape Pos a37) (@Nil Shape Pos (Op Shape
+                                                                                          Pos))
+              | add0 a39 a40 =>
+                  @append Shape Pos (Op Shape Pos) (@append Shape Pos (Op Shape Pos) (a39 >>=
+                                                                                      (fun (a39_0 : Expr Shape Pos) =>
+                                                                                         comp_0 Shape Pos a39_0)) (a40
+                                                                                      >>=
+                                                                                      (fun (a40_0 : Expr Shape Pos) =>
+                                                                                         comp_0 Shape Pos a40_0)))
+                                                   (@Cons Shape Pos (Op Shape Pos) (ADD Shape Pos) (@Nil Shape Pos (Op
+                                                                                     Shape Pos)))
+              end.
+
+Definition comp (Shape : Type) (Pos : Shape -> Type) (a36
+    : Free Shape Pos (Expr Shape Pos))
+   : Free Shape Pos (Code Shape Pos) :=
+  a36 >>= (fun (a36_0 : Expr Shape Pos) => comp_0 Shape Pos a36_0).
+
+Definition prop_comp_comp'_eq (Shape : Type) (Pos : Shape -> Type) (e
+    : Free Shape Pos (Expr Shape Pos))
+   : Free Shape Pos (Property Shape Pos) :=
+  @eqProp Shape Pos (Code Shape Pos) (comp Shape Pos e) (comp' Shape Pos e).
+
+Definition prop_comp_correct (Shape : Type) (Pos : Shape -> Type) (P
+    : Partial Shape Pos) (e : Free Shape Pos (Expr Shape Pos))
+   : Free Shape Pos (Property Shape Pos) :=
+  @eqProp Shape Pos (Stack Shape Pos) (exec Shape Pos P (comp Shape Pos e) (@Nil
+                                             Shape Pos (Integer Shape Pos))) (@Cons Shape Pos (Integer Shape Pos) (eval
+                                                                                                                   Shape
+                                                                                                                   Pos
+                                                                                                                   e)
+                                                                                                                  (@Nil
+                                                                                                                   Shape
+                                                                                                                   Pos
+                                                                                                                   (Integer
+                                                                                                                    Shape
+                                                                                                                    Pos))).
